Schnorr from abstract to more concrete

proof/schnorr_protocol/Zp_SchnorrProtocol.ec
@@ -13,46 +13,46 @@ require ZModPStar.
 require import Ring_ops_spec.
 import Zp.
 
-op p = Zp.p.
+clone ZModPStar as ZPS with op p <- Zp.p,
+                            theory Zp <= Zp
+rename "zmod" as "zp".
+
+
+import ZPS.
+
+op g : ZPS.zp.
 op q : int.
 axiom q_prime : prime q.
+axiom g_unit : unit g.
+axiom g_q_assumption: (ZModpField.exp g q) = Zp.one.
 
-clone ZModPStar as ZPS
-with op p = p,
-     theory Zp <= Zp
-proof ge2_p.
-  (* TODO proof* *)
-realize ge2_p. admit. qed.
+lemma lll' (z : zp) : unit z => forall x, 0 <= x => Zps.(^) (Sub.insubd z)  x = Sub.insubd (ZModpField.exp z x). 
+move => z_unit. apply intind. progress. smt. progress.  timeout 20. smt.
+qed.
 
-(* G := ZPS.zmods is the group with operate in *)
-  
-op g : ZPS.zmods.
-  
 clone import Abstract_SchnorrProtocol as LSP with
+  op g <- Sub.insubd g,
   op q <- q,
-  theory CG <- ZPS.Zps.
-  (* TODO proof* *)
-  
-type statement = LSP.statement.           (* statement *)
-type witness  = LSP.witness.          (* witness *)
-type commitment = LSP.commitment.            (* commitment *)
-type response = LSP.response.          (* response *)
-type challenge = LSP.challenge.          (* challenge *)
-type secret  = EG.zmod.
+  theory CG <- ZPS.Zps
+proof g_is_generator, q_prime.
+realize g_is_generator.  rewrite lll'. apply g_unit. smt(q_prime).
+rewrite g_q_assumption. auto. qed.
+realize q_prime.  apply q_prime. qed.
 
-  (* Multiplication in Zq *)
-op ( * ) = EG.( * ).
-  (* Addition in Zq *)
-op ( + ) = EG.( + ).
-  (* Multiplication in G = Zq* *)
-op ( ** ) = ZPS.Zps.( * ).
-op ( ^^ ) = ZPS.Zps.( ^ ).
+
+
+
+type statement   = zp.           (* statement *)
+type witness     = int.          (* witness *)
+type commitment  = zp.            (* commitment *)
+type response    = int.          (* response *)
+type challenge   = int.          (* challenge *)
+type secret      = int.
 
 module type ZKProverG = {
   proc commitment() : commitment * secret
   proc response(w : witness, r : secret, c : challenge) : response
 }.
-
 
 module type ZKVerifierG = {
   proc challenge() : challenge
@@ -60,12 +60,11 @@ module type ZKVerifierG = {
     bool
 }.
 
-
 module SchnorrProver : ZKProverG = {
   proc commitment() : commitment * secret = {
     var r : secret;
-    r <$ (* [0..p-2] *) witness; (* TODO: pick from challenge set *)
-    return (g ^^ r, r);
+    r <$ [0..q-1]; 
+    return (ZModpField.exp g r, r);
   }
   proc response(w: witness, r:secret, c: challenge) : response = {
     return r + c * w;
@@ -76,11 +75,11 @@ module SchnorrProver : ZKProverG = {
 module SchnorrVerifier : ZKVerifierG = {
   proc challenge() : challenge = {
     var c;
-    c <$ (* [0..p-2] *) witness; (* TODO: pick from challenge set *)
+    c <$ [0..q-1];
     return c;
   }
   proc verify(s: statement, z: commitment, c: challenge, t: response) : bool = {
-    return (z ** (s ^^ c) = g ^^ t) /\ s ^^ q = ZPS.Zps.e;
+    return ((ZModpField.exp g t) = (s ^^ c) * z) /\ (ZModpField.exp s q) = Zp.one;
   }
 }.
 
@@ -98,36 +97,158 @@ module CompletenessG(P : ZKProverG, V : ZKVerifierG) = {
 
 
 
-axiom exp_lemma4 : forall (x : zp) (n : int),  (x ^^ n) = Sub.val ((Sub.insubd x) ^^ n).
-lemma bbb : forall (a b : zmods), (Sub.val a = Sub.val b) <=> (a = b). smt. qed.
+op completeness_relationG (s:statement) (w:witness) = (ZModpField.exp g w) = s.
 
-lemma completenessG (s : statement) (w : witness) &m: LSP.completeness_relation (Sub.insubd s) w =>
-  Pr[ CompletenessG(SchnorrProver, SchnorrVerifier).main(s,w)@&m : res] = 1%r.
+
+lemma exp_lemma6 (z : zp) : unit z => forall n,  unit (z ^^ n).
+progress. apply ZModpRing.unitrX. auto.
+qed.
+
+
+
+
+
+
+lemma lll'' (z : zp) : unit z => forall x, x < 0 => Zps.(^) (Sub.insubd z) x = Zps.inv (Zps.(^) (Sub.insubd z) (- x)).
+smt().
+qed.
+
+
+lemma lll (z : zp) : unit z => forall x, Zps.(^) (Sub.insubd z)  x = Sub.insubd (ZModpField.exp z x). 
+move => zu.
+move => x.
+case (0 <= x).  apply lll'. auto.
+move => xl.
+rewrite lll''. auto. smt().
+rewrite lll'. auto. smt().
+smt(@ZModpField @Sub).       
+qed.
+
+lemma bbb : forall (a b : zps), (Sub.val a = Sub.val b) <=> (a = b). smt. qed.
+
+lemma completeness_relation_compatible : forall s w, completeness_relationG s w => completeness_relation (Sub.insubd s) (EG.inzmod w).
+move => s w h. rewrite /completeness_relationG /completeness_relation /IsDL /=. (* move => eq. *)
+rewrite /(^^).
+rewrite EG.inzmodK.
+rewrite - pow_mod. 
+rewrite lll. apply g_unit. auto.
+rewrite - bbb.
+rewrite - h. auto.
+qed.
+
+
+
+
+lemma llll (x y : zp) : unit x => unit y => (Zps.( * ) (Sub.insubd x)  (Sub.insubd y) )= Sub.insubd (x * y).
+progress. smt. qed.
+
+lemma exp_lemma4 : forall (x : zp) (n : int), unit x => (ZModpField.exp x q) = one =>  (x ^^ n) = Sub.val ((Sub.insubd x) ^^ (EG.inzmod n)). 
+proof. progress. rewrite /(^^). rewrite lll. auto.
+rewrite  EG.inzmodK.
+have ->: (ZModpField.exp x (n %% q)) = (ZModpField.exp x n). smt.
+rewrite Sub.insubdK.
+smt.
+auto.
+qed.
+
+
+lemma exp_lemma5 : forall (z : zp) (n : int), unit z => 0 <= n => (ZModpField.exp z q) = one  => Sub.insubd z ^^ (EG.inzmod n) = (Zps.(^) (Sub.insubd z) n).
+progress. rewrite /(^^). 
+rewrite lll. auto. 
+rewrite - bbb.
+rewrite Sub.insubdK. rewrite /P. smt.
+have ->: (EG.asint ((EG.inzmod n))%EG) = n %% q. smt.
+rewrite lll. auto.  
+rewrite Sub.insubdK. smt.
+rewrite  (exp_mod' z n q _). auto. auto.
+qed.
+
+
+   
+
+
+lemma nosmt dokas : forall s w, s = ZModpField.exp g w => ZModpField.exp s q = one.
+progress. 
+have ->: (ZModpField.exp ((ZModpField.exp g w)) q) = (((ZModpField.exp g (w * q)))). 
+ rewrite - ZModpField.exprM. auto.
+have -> : w * q = q * w. smt().
+have ->: (ZModpField.exp g (q * w)) = (ZModpField.exp ((ZModpField.exp g q)) w).
+rewrite  ZModpField.exprM. auto.
+rewrite  g_q_assumption. smt(@ZModpField).
+qed.
+
+(* in completeness not needed for any q, but only for THE q *)
+
+lemma completenessG (s : statement) (w : witness) &m: completeness_relationG s w =>
+   Pr[ CompletenessG(SchnorrProver, SchnorrVerifier).main(s,w)@&m : res] = 1%r.
 proof. progress.
-rewrite - (LSP.dl_completeness (Sub.insubd s) w &m). auto.
+have statement_not_zero : unit s. rewrite - H. apply exp_lemma6. apply g_unit.
+rewrite /completeness_relation /IsDL in H.
+rewrite - (LSP.dl_completeness (Sub.insubd s) (EG.inzmod w) &m). 
+  apply completeness_relation_compatible. auto.
 byequiv (_: _ ==> _). proc.
 inline*. wp. 
-rnd. wp. rnd.  wp. skip. progress.  admit.
-admit. rewrite /verify_transcript. simplify. rewrite /(^^). 
-have f : ((s{1} ^^ q) = one) =  ((Sub.insubd s{1}) ^^ q = (Sub.insubd one)).
-rewrite exp_lemma4. 
-rewrite - (bbb ( ((Sub.insubd s{1})%Sub ^^ q)) (Sub.insubd one)). 
+rnd EG.inzmod EG.asint. wp. rnd EG.inzmod EG.asint. wp. skip. progress. smt(@EG). smt(@DInterval @EG).
+rewrite EG.inzmodK. 
+ have : 0 <= r0L < q. smt(@DInterval @List). 
+smt(@IntDiv).
+smt(@EG).
+smt(@DInterval @EG).
+smt(@DInterval @EG).
+have -> :((s{1} ^^ q) = one) =  ((Sub.insubd s{1}) ^^ (EG.inzmod q) = (Sub.insubd one)).
+rewrite exp_lemma4. auto. rewrite (dokas s{1} w{1}). rewrite - H. auto. auto.
+rewrite - (bbb ( ((Sub.insubd s{1})%Sub ^^ (EG.inzmod q))) (Sub.insubd one)). 
 have -> : (Sub.val ((Sub.insubd one))%Sub) = one. 
-rewrite Sub.insubdK. smt. auto. auto. simplify.
-have ->: ((g ^^ r0L)%ZModpRing * (s{1} ^^ c0L)%ZModpRing = (g ^^ (r0L + c0L * w{2}))%ZModpRing)  
-
-  = ((Sub.Lift.lift2 Zp.( * ) ((Sub.insubd s{1})%Sub ^^ (EG.asint c0L)%EG)%CG
-    ((Sub.insubd g)%Sub ^^ (EG.asint r0L)%EG)%CG) = ((Sub.insubd g)%Sub ^^ (EG.asint (r0L + c0L * w{2})%EG)%EG)%CG).
-
+rewrite Sub.insubdK. smt(@Zp). auto. auto. simplify. rewrite /verify_transcript. simplify.
+have ->: ((g ^^ (r0L + c0L * w{1})) = (s{1} ^^ c0L) * (g ^^ r0L))  
+  = ((Sub.insubd g)%Sub ^^ (EG.(+) (EG.inzmod r0L) (EG.( * ) (EG.inzmod c0L)  (EG.inzmod w{1})))%EG =
+ (Sub.Lift.lift2 Zp.( * ) ((Sub.insubd s{1})%Sub ^^ (EG.inzmod c0L)%EG)
+    ((Sub.insubd g)%Sub ^^ (EG.inzmod r0L)%EG))%Sub.Lift ).
+rewrite /lift2. 
+rewrite exp_lemma4. apply g_unit. apply g_q_assumption.
+rewrite exp_lemma4. assumption. rewrite (dokas s{1} w{1}). rewrite - H. auto. auto.
+rewrite exp_lemma4. apply g_unit. apply g_q_assumption.
+simplify.
+have ->: (EG.inzmod (r0L + c0L * w{1})) 
+ = (EG.(+) (EG.inzmod r0L) (EG.( * ) (EG.inzmod c0L)  (EG.inzmod w{1}))). smt(@EG).
 rewrite - bbb.
-smt.
-simplify. admit. auto. auto.
+ pose x := (Sub.val ((Sub.insubd g)%Sub ^^ (EG.(+) (EG.inzmod r0L) (EG.( * ) (EG.inzmod c0L) (EG.inzmod w{1}))))).
+rewrite Sub.insubdK. rewrite /P. smt.
+rewrite - exp_lemma4. assumption. rewrite (dokas s{1} w{1}). rewrite - H. auto. auto. rewrite - exp_lemma4.  apply g_unit. apply g_q_assumption.
+auto.
+pose x := (Sub.insubd g)%Sub ^^ (EG.(+) (EG.inzmod r0L) (EG.( * ) (EG.inzmod c0L)  (EG.inzmod w{1})))%EG.
+pose z := Sub.insubd s{1}.
+pose o := Sub.insubd one.
+rewrite /Zp.( * ).
+pose y := (Sub.Lift.lift2 Ring_ops_spec.Zp.( * ) ((Sub.insubd s{1})%Sub ^^ (EG.inzmod c0L)%EG)
+    ((Sub.insubd g)%Sub ^^ (EG.inzmod r0L)%EG)).
+rewrite exp_lemma5. assumption. smt(@DInterval).
+rewrite - H. 
+  have ->: (ZModpField.exp ((ZModpField.exp g w{1})) q) = (((ZModpField.exp g (w{1} * q)))). 
+   rewrite - ZModpField.exprM. auto.
+  have -> : w{1} * q = q * w{1}. smt().
+  have ->: (ZModpField.exp g (q{1} * w{1})) = (ZModpField.exp ((ZModpField.exp g q{1})) w{1}).
+  rewrite  ZModpField.exprM. auto.
+  rewrite g_q_assumption. smt(@ZModpField).
+timeout 20. 
+rewrite /(^^).
+have ->: Zps.(^) z ((EG.asint ((EG.inzmod q)))) = Zps.(^) z q. 
+rewrite  EG.inzmodK. 
+  have ->: (q %% q) = 0. smt(@IntDiv).
+  have ->: Zps.(^) z 0 = (Sub.insubd one). smt(@Zps).
+  rewrite /z. rewrite lll. assumption. 
+  rewrite (dokas s{1} w{1}). rewrite - H. auto. auto. auto.
+auto. auto.
 qed.
+
+
+
 
 
 
 (* Extractability  *)
 import Rew.
+
 op sec_to_sbits : secret -> sbits.
 op sec_from_sbits : sbits -> secret.
 axiom sec_enc x : x = sec_from_sbits (sec_to_sbits x).
@@ -164,21 +285,22 @@ module type ExtractorG(P: ZKRewindableMaliciousProverG) = {
 }.
 
 module SpecialSoundnessAdversaryG(P : ZKRewindableMaliciousProverG)  = {
-  proc attack(statement:statement):transcript * transcript = {
+  proc attack(statement:statement):(commitment * int * response) * (commitment * int * response) = {
     var i,c1,c2,r1,r2,pstate;
     i <@ P.commitment();
-    c1 <$ [0..p-2];
+    c1 <$ [0..q-1];
     pstate <@ P.getState();
     r1 <@ P.response(c1);
-    c2 <$ [0..p-2];
+    c2 <$ [0..q-1];
     P.setState(pstate);
     r2 <@ P.response(c2);
     return ((i,c1,r1), (i,c2,r2));
   }
 }.
 
+
 op special_soundness_extractG (t1 t2 : commitment * challenge * response): witness = 
- (special_soundness_extract witness t1 t2).
+ EG.asint (special_soundness_extract witness (Sub.insubd t1.`1, EG.inzmod t1.`2, EG.inzmod t1.`3) (Sub.insubd t2.`1, EG.inzmod t2.`2,EG.inzmod t2.`3)).
 
 module (ExtractorG : ExtractorG)(P : ZKRewindableMaliciousProverG) = {  
   module SA = SpecialSoundnessAdversaryG(P)
@@ -207,44 +329,150 @@ declare axiom rewindable_P_plus :
 
 
 
+
 local module P' = {
   proc commitment(s : dl_stat) : dl_com  = {
     var r;
     r <@ P.commitment();
-    return r;
+    return (Sub.insubd r);
   }  
   proc response(challenge : dl_chal) : dl_resp  = {
     var r;
-    r <@ P.response(challenge);
-    return r;
+    r <@ P.response( EG.asint challenge);
+    return (EG.inzmod r);
   }  
   proc getState = P.getState
   proc setState = P.setState
 }.
 
 
-lemma extractabilityG &m s: 
-  Pr[ExtractorG(P).extract(s) @ &m : soundness_relation s res ] >=
-   (Pr[SoundnessG(P, SchnorrVerifier).run(s) @ &m : res] ^ 2
-       - 1%r / (size (range 0 (p - 1)))%r
+
+lemma lles (a b : real) : 0%r <= a <= 1%r => 0%r <= b <= 1%r 
+  => a  <= b  =>  a ^ 2 <= b ^ 2.
+smt(@RealOrder).
+qed.
+
+lemma lles2 (a b x y : real) : 0%r <= a <= x => 0%r <= b <= y
+  => a * b <= x * y.
+smt(@Real @RealOrder).
+qed.
+
+lemma lles3 (a b : real) : 0%r < a => 0%r <= a * b => 0%r <= b.
+progress.
+smt(@Real @RealOrder).
+qed.
+
+lemma extractabilityG &m (s : zp): 
+  Pr[ExtractorG(P).extract(s) @ &m : LSP.soundness_relation (Sub.insubd s) (EG.inzmod res) ] >=
+  (Pr[SoundnessG(P, SchnorrVerifier).run(s) @ &m : res] ^ 2
+       - 1%r / (size EG.DZmodP.Support.enum)%r
            * Pr[SoundnessG(P, SchnorrVerifier).run(s) @ &m : res]).
-proof.
-have -> : Pr[SoundnessG(P, SchnorrVerifier).run(s) @ &m : res]
- = Pr[Soundness(P', HV).run(s) @ &m : res].
-byequiv (_: ={glob P, arg} ==> _).
+proof. 
+(* s = zero *)
+case (s = zero). move => s_is_zero.
+  have ->: Pr[SoundnessG(P, SchnorrVerifier).run(s) @ &m : res] = 0%r.
+  pose ss := s.
+  byphoare (_: arg = s ==> _). proc. hoare.
+  inline*. wp.  call (_:true). wp. rnd. call(_:true). skip. progress. rewrite s_is_zero. 
+  have ->: ZModpField.exp zero  q = zero. 
+    rewrite (ZModpField.expr0z q). smt(q_prime).
+  smt(@Zp). auto. auto. simplify.
+  have ->: 0%r ^ 2 = 0%r. smt(@Real). 
+  rewrite Pr[mu_ge0]. auto.
+(* s <> zero *)
+move => s_not_zero.
+have soundness_less : Pr[SoundnessG(P, SchnorrVerifier).run(s) @ &m : res]
+ <= Pr[Soundness(P', HV).run(Sub.insubd s) @ &m : res].
+byequiv (_: _ ==> _).
 proc. inline*. wp.  call(_:true). wp. 
-rnd. wp.  call (_:true). wp.  skip. progress.
-smt(@Distr). clear H H0. rewrite /verify_transcript. simplify. smt(@Zp). auto. auto. 
-have -> : Pr[ExtractorG(P).extract(s) @ &m : soundness_relation s res] 
- = Pr[Extractor(P').extract(s) @ &m : soundness_relation s res].
-byequiv (_: ={glob P, arg} ==> _). proc.
+rnd EG.inzmod EG.asint. wp. call (_:true). wp. skip. progress.
+smt(@EG).  
+smt(@DInterval @EG).
+smt(@DInterval @EG).  
+(* result_R = zero *)
+case (result_R = Zp.zero). 
+move => result_R_zero. smt.
+(* result_R <> zero  *)
+move => commitment_non_zero.
+have f: ((g ^^ result_R0) = (s{1} ^^ c0L) * result_R)
+             => ((Sub.insubd g)%Sub ^^ (EG.inzmod result_R0)%EG =
+ (Sub.Lift.lift2 Ring_ops_spec.Zp.( * ) ((Sub.insubd s{1})%Sub ^^ (EG.inzmod c0L)%EG)
+    ((Sub.insubd result_R)))%Sub.Lift ).
+rewrite /lift2.
+rewrite exp_lemma4. apply g_unit. apply g_q_assumption.
+rewrite exp_lemma4. apply unitE. assumption. assumption.
+simplify.
+rewrite - bbb.
+pose x := (Sub.val ((Sub.insubd g)%Sub ^^ (EG.inzmod result_R0))).
+rewrite Sub.insubdK.
+rewrite - exp_lemma4. apply unitE. assumption. assumption. 
+rewrite /P.
+  have ->: (Sub.val ((Sub.insubd result_R))%Sub) = result_R. 
+    rewrite Sub.insubdK. apply unitE. assumption. auto.
+    smt.
+rewrite - exp_lemma4. apply unitE. assumption. assumption.
+rewrite Sub.insubdK. smt(@Ring_ops_spec.Zp). auto.
+apply f. auto.
+rewrite - bbb.
+      (* TODO *)
+rewrite -  exp_lemma5. apply unitE. assumption. smt(@DInterval). assumption.
+timeout 20. smt. 
+auto.
+auto.
+have -> : Pr[ExtractorG(P).extract(s) @ &m : soundness_relation (Sub.insubd s)  (EG.inzmod res)] 
+ = Pr[Extractor(P').extract(Sub.insubd s) @ &m : soundness_relation (Sub.insubd s) res].
+byequiv (_: _ ==> _). proc.
 inline*. wp. call (_:true). wp. 
-call (_:true). wp.  rnd. wp. call (_:true). wp.
-call (_:true). rnd. wp.  call (_:true). wp.  skip. progress. auto. auto. 
-apply (dl_statistical_PoK P' _ _ _ &m s).
+call (_:true). wp. 
+rnd EG.inzmod EG.asint. wp. call (_:true). wp.
+call (_:true). rnd EG.inzmod EG.asint. wp.  call (_:true). wp.  skip. progress. 
+smt. smt(@DInterval @EG). smt(@EG @DInterval). smt(@EG @DInterval).
+have -: LSP.soundness_relation ((Sub.insubd p{1}))%Sub
+      ((EG.inzmod
+          (special_soundness_extractG (result_R, c1L, result_R1)
+             (result_R, c2L, result_R2))))%EG.
+auto. clear H9.
+rewrite /soundness_relation /IsDL /special_soundness_extract. simplify.
+rewrite /special_soundness_extractG. simplify. rewrite /special_soundness_extract.
+simplify. smt.
+have -: soundness_relation ((Sub.insubd p{1}))%Sub
+      (special_soundness_extract ((Sub.insubd p{1}))%Sub
+         ((Sub.insubd result_R)%Sub, (EG.inzmod c1L)%EG, (EG.inzmod result_R1)%EG)
+         ((Sub.insubd result_R)%Sub, (EG.inzmod c2L)%EG, (EG.inzmod result_R2)%EG)). auto.
+rewrite /soundness_relation /IsDL /special_soundness_extract. simplify.
+rewrite /special_soundness_extractG. simplify. rewrite /special_soundness_extract.
+simplify. smt.
+auto. auto.
+have  :   Pr[Soundness(P', HV).run((Sub.insubd s)%Sub) @ &m : res] ^ 2 -
+  1%r / (size EG.DZmodP.Support.enum)%r *
+  Pr[Soundness(P', HV).run((Sub.insubd s)%Sub) @ &m : res] <=
+  Pr[Extractor(P').extract((Sub.insubd s)%Sub) @ &m :
+     soundness_relation ((Sub.insubd s))%Sub res]. 
+apply (dl_statistical_PoK P' _ _ _ &m (Sub.insubd s)).
 proc. call P_response_ll. auto.
 proc. call P_commitment_ll. auto.
 apply rewindable_P_plus.
+pose a:= Pr[Soundness(P', HV).run((Sub.insubd s)) @ &m : res].
+pose b:= Pr[Extractor(P').extract((Sub.insubd s)%Sub) @ &m :
+   soundness_relation ((Sub.insubd s))%Sub res].
+pose c := (size EG.DZmodP.Support.enum)%r.
+pose q := Pr[SoundnessG(P, SchnorrVerifier).run(s) @ &m : res].
+progress.
+case ((q ^ 2 - q / c) <= 0%r). smt.
+move => pos. have impfact :  0%r < q * (q - 1%r / c). timeout 10. smt(@Real @RealOrder).
+have : q <= a. auto. move => aq.
+have ls1 : 0%r <= a <= 1%r. smt.
+have ls2 : 0%r <= q <= 1%r. smt.
+have : q ^ 2 - q / c  <=  a ^ 2 - a / c .
+ have ->: q ^ 2 - q/c = q * (q  - 1%r/c). smt(@Real).
+ have ->: a ^ 2 - a/c = a * (a  - 1%r/c). smt(@Real).
+ have z: (q - 1%r / c) <= (a - 1%r / c). smt(@Real).
+ apply lles2.  split. smt(@Real @RealOrder).
+auto. 
+split. 
+apply (lles3 q). smt(@Real @RealOrder). smt(@Real @RealOrder).
+auto.
+smt(@Real @RealOrder).
 qed.
 
 end section.
